eve/Src/framework/eiffel2boogie/tests/framing/ownership/iterator/f_i_iterator_d.e
@@ -20,6 +20,7 @@ feature
 			t.is_wrapped -- default: creator
 			across t.observers as o all o.item.is_wrapped end -- default: creator
 			t /= Void
+			across t.observers as ic all ic.item.generating_type = {F_I_ITERATOR_D} end
 
 			modify (Current)
 			modify_field ("observers", t)
